ghc/CmmExpr.v
@@ -1,5 +1,6 @@
 (* Coq implementation of compiler/cmm/CmmExpr.hs *)
 Require Import BinNums.
+Require Import List.
 
 Require Import GHC.CmmType.
 Require Import GHC.Int.
@@ -45,7 +46,6 @@ Inductive CLabel := nat.
 Inductive CmmLit : Set :=
 | CmmInt: Integer -> Width -> CmmLit
 | CmmFloat: Rational -> Width -> CmmLit
-| CmmVec: list CmmLit -> CmmLit
 | CmmLabel: CLabel -> CmmLit
 | CmmLabelOff: CLabel -> Int -> CmmLit
 | CmmLabelDiffOff: CLabel -> CLabel -> Int -> Width -> CmmLit
@@ -61,3 +61,46 @@ Inductive CmmExpr : Set :=
 | CE_CmmStackSlot: Area -> Int -> CmmExpr
 | CE_CmmRegOff : CmmReg -> Int -> CmmExpr
 .
+
+Definition cmmLabelType (lbl:CLabel) : CmmType := bWord.
+
+Definition cmmLitType (l : CmmLit) : CmmType :=
+  match l with
+  | CmmInt _ width => cmmBits width
+  | CmmFloat _ width => cmmFloat width
+  | CmmLabel lbl => cmmLabelType lbl
+  | CmmLabelOff lbl _ => cmmLabelType lbl
+  | CmmLabelDiffOff _ _ _ width => cmmBits width
+  | CmmBlock _ => bWord
+  | CmmHighStackMark => bWord
+  end.
+
+Definition localRegType (l:LocalReg) : CmmType :=
+  match l with
+  | LR_LocalReg _ rep => rep
+  end.
+
+Definition globalRegType (g:GlobalReg) : CmmType :=
+  match g with
+  | VanillaReg _ _ => bWord (* we might want to look at the second parameter *)
+  | FloatReg _ => cmmFloat W32
+  | DoubleReg _ => cmmFloat W64
+  | LongReg _ => cmmBits W64
+  | _ => bWord
+  end.
+                                         
+Definition cmmRegType (r:CmmReg) : CmmType :=
+  match r with
+  | CmmLocal reg => localRegType reg
+  | CmmGlobal reg => globalRegType reg
+  end.
+
+Fixpoint cmmExprType (e : CmmExpr) : CmmType :=
+  match e with
+  | CE_CmmLit lit => cmmLitType lit
+  | CE_CmmLoad _ rep => rep
+  | CE_CmmReg reg => cmmRegType reg
+  | CE_CmmMachOp op args => machOpResultType op (List.map cmmExprType args)
+  | CE_CmmStackSlot _ _ => bWord
+  | CE_CmmRegOff reg _ => cmmRegType reg
+  end.
