ghc/CmmMachOp.v
@@ -13,3 +13,15 @@ Inductive MachOp :=
 Definition MachOp_eq_dec (m1 m2 : MachOp) : {m1 = m2} + {m1 <> m2}.
   decide equality; try (apply Width_eq).
 Defined.
+
+Definition comparisonResultRep := bWord. (* but Haskellers are not sure about it :-) *)
+                                    
+Definition machOpResultType (mo:MachOp) (tys:list CmmType) : CmmType :=
+  match mo with
+  | MO_Add r => cmmBits r (* should be type of first argument
+                             if we are interested in GC-ptr-hood of values *)
+  | MO_Sub r => cmmBits r (* same as above *)
+  | MO_Mul r => cmmBits r
+  | MO_Eq _ => comparisonResultRep
+  | MO_Ne _ => comparisonResultRep
+  end.
